VCG.thy
@@ -18,18 +18,44 @@ lemma hoare_intro:
 
 section "Annotations"
 
-type_synonym block_preconditions = "(llvm_label * (state \<Rightarrow> bool)) list"
-type_synonym function_postcondition = "(llvm_value * state) \<Rightarrow> bool"
+type_synonym block_preconditions = "(llvm_identifier * (state \<Rightarrow> bool)) list"
+type_synonym function_postcondition = "(llvm_value option * state) \<Rightarrow> bool"
 datatype annotated_function = annotated "llvm_function" "block_preconditions" "function_postcondition"
 
-partial_function (tailrec) execute_blocks_from_until :: "annotated_function \<Rightarrow> llvm_label \<Rightarrow> llvm_label option \<Rightarrow> state \<Rightarrow> (state * llvm_block_return) result" where
+
+inductive verify where
+  return:
+    "map_of blocks label = Some block \<Longrightarrow>
+    execute_block prev block s = ok (s', return_value v) \<Longrightarrow>
+    post (Some v, s') \<Longrightarrow>
+    verify (annotated (func fdef blocks) pre post) prev label s (s', return_value v)"
+| branch_precond:
+    "map_of blocks label = Some block \<Longrightarrow>
+    execute_block prev block s = ok (s', branch_label bl) \<Longrightarrow>
+    map_of pre bl = Some precond \<Longrightarrow>
+    precond s' \<Longrightarrow>
+    \<forall>s. precond s \<longrightarrow> verify (annotated (func fdef blocks) pre post) (Some label) bl s (s'', r') \<Longrightarrow>
+    verify (annotated (func fdef blocks) pre post) prev label s (s'', r')"
+| branch_without:
+    "map_of blocks label = Some block \<Longrightarrow>
+    execute_block prev block s = ok (s', branch_label bl) \<Longrightarrow>
+    map_of pre bl = None \<Longrightarrow>
+    verify (annotated (func fdef blocks) pre post) (Some label) bl s (s'', r') \<Longrightarrow>
+    verify (annotated (func fdef blocks) pre post) prev label s (s'', r')"
+
+
+
+term verify
+
+
+partial_function (tailrec) execute_blocks_from_until :: "annotated_function \<Rightarrow> llvm_identifier \<Rightarrow> llvm_identifier option \<Rightarrow> state \<Rightarrow> (state * llvm_block_return) result" where
   "execute_blocks_from_until fun label prev s = (case fun of annotated (func fdef blocks) pre post \<Rightarrow>
     (case map_of blocks label of
       None \<Rightarrow> err unknown_label
     | Some b \<Rightarrow> (case (execute_block prev b s) of
-        ok (s', return_value v) \<Rightarrow> ok (s', return_value v)
+        ok (s', return_value v) \<Rightarrow> ok (s', return_value v) \<comment> \<open>function terminated execution\<close>
       | ok (s', branch_label l) \<Rightarrow> (case map_of pre l of
-          Some _ \<Rightarrow> ok (s', branch_label l)
+          Some _ \<Rightarrow> ok (s', branch_label l)                \<comment> \<open>block terminated execution\<close>
         | None \<Rightarrow> execute_blocks_from_until fun l (Some label) s'
         )
       | err e \<Rightarrow> err e
@@ -38,13 +64,48 @@ partial_function (tailrec) execute_blocks_from_until :: "annotated_function \<Ri
   )"
 lemmas [code] = execute_blocks_from_until.simps
 
-fun block_transitions :: "llvm_labeled_blocks \<Rightarrow> (llvm_label * llvm_label) list" where
+lemma [partial_function_mono]:
+"monotone tailrec.le_fun tailrec_ord
+          (\<lambda>f. wp (execute_blocks_from_until (annotated fun pres post) current prev s)
+                 (\<lambda>(s', y).
+                     case_llvm_block_return (\<lambda>v. x3 (Some v, s'))
+                      (\<lambda>l'. case map_of x2 l' of None \<Rightarrow> False
+                             | Some Q \<Rightarrow> Q s' \<and> f (((annotated fun pres post, l'), Some current), s'))
+                      y))"
+  unfolding wp_gen_def fun_ord_def
+  apply (rule monotoneI)
+  apply (auto split: result.splits llvm_block_return.splits option.splits simp: Partial_Function.tailrec.leq_refl)
+  subgoal for f g r s h l pre
+    by (cases "pre (r,s,h)", auto simp: Partial_Function.tailrec.leq_refl)
+  done
+
+partial_function (tailrec)  wp_blocks_from_until where "wp_blocks_from_until fun l p s =
+  (case fun of annotated (func fdef blocks) pre post \<Rightarrow>
+    (if (the (map_of pre l) s)
+       then
+    (wp (execute_blocks_from_until (annotated (func fdef blocks) pre post) l p s)
+      (\<lambda>(s,r).
+        case r of
+          return_value v \<Rightarrow> post (Some v, s) \<comment> \<open>postcondition of whole annotated function holds\<close>
+        | branch_label l' \<Rightarrow>            \<comment> \<open>look at precondition of next block and prove that\<close>
+            (case (map_of pre l') of
+                   \<comment> \<open>next block has a precondition;  we recurse\<close>
+                   Some Q \<Rightarrow> Q s \<and> wp_blocks_from_until fun l' (Some l) s
+                 | None \<Rightarrow> False))
+      )
+       else False))"
+  
+
+(* NOTE edo this may be a coinductive definition *)
+
+
+fun block_transitions :: "llvm_labeled_blocks \<Rightarrow> (llvm_identifier * llvm_identifier) list" where
   "block_transitions ((from, (_, _, br_label to)) # bs) = (from, to) # block_transitions bs"
 | "block_transitions ((from, (_, _, br_i1 _ to1 to2)) # bs) = (from, to1) # (from, to2) # block_transitions bs"
 | "block_transitions (_#bs) = block_transitions bs"
 | "block_transitions [] = []"
 
-fun transitions_to :: "(llvm_label * llvm_label) list \<Rightarrow> llvm_label list \<Rightarrow> (llvm_label option * llvm_label) list" where
+fun transitions_to :: "(llvm_identifier * llvm_identifier) list \<Rightarrow> llvm_identifier list \<Rightarrow> (llvm_identifier option * llvm_identifier) list" where
   "transitions_to ((from, to)#ls) l = (if List.member l to then (Some from,to)#transitions_to ls l else transitions_to ls l)"
 | "transitions_to [] _ = []"
 
@@ -87,7 +148,7 @@ fun verify_blocks_hoare where
       precond
       (execute_blocks_from_until (annotated (func fdef blocks) pre post) label prev)
       (\<lambda>(s, r). (case r of
-        return_value v \<Rightarrow> post (v, s)
+        return_value v \<Rightarrow> post (Some v, s)
       | branch_label l \<Rightarrow> (case map_of pre l of
           Some Q \<Rightarrow> Q s
         | None \<Rightarrow> False
@@ -103,7 +164,7 @@ fun verify_blocks where
   "verify_blocks f ((prev, label)#ls) = (verify_blocks_from f label prev \<and> verify_blocks f ls)"
 | "verify_blocks _ [] = True"
 
-fun verify_function where
+fun verify_function :: "annotated_function \<Rightarrow> bool" where
   "verify_function (annotated (func fdef ((first_label, first_block)#bs)) pre post) = (
     distinct (map fst pre)
   \<and> verify_blocks
@@ -113,7 +174,37 @@ fun verify_function where
         (if List.member (map fst pre) first_label then map fst pre else first_label#(map fst pre))
       ))
   )"
-| "verify_function _ = True"
+| "verify_function (annotated _ pre post) = False"
+
+
+
+section "Useful Shorthands"
+
+find_theorems "_ \<and> True"
+
+definition register_contains_value :: "llvm_identifier \<Rightarrow> llvm_value \<Rightarrow> state \<Rightarrow> bool" where
+  "register_contains_value n v s \<equiv> register_\<alpha> s (reg n) = Some v"
+
+definition register_contains_allocated_address :: "llvm_identifier \<Rightarrow> state \<Rightarrow> bool" where
+  "register_contains_allocated_address n s \<equiv> \<exists>a. register_\<alpha> s (reg n) = Some (addr a) \<and> memory_\<alpha> s a \<noteq> None"
+
+definition register_contains_address_with_value :: "llvm_identifier \<Rightarrow> llvm_value \<Rightarrow> state \<Rightarrow> bool" where
+  "register_contains_address_with_value n v s \<equiv> \<exists>a. register_\<alpha> s (reg n) = Some (addr a) \<and> memory_\<alpha> s a = Some (Some v)"
+
+fun unique_address :: "llvm_address \<Rightarrow> llvm_address list \<Rightarrow> bool" where
+  "unique_address ad (a#as) = ((ad \<noteq> a) \<and> unique_address ad as)"
+| "unique_address _ [] = True"
+
+fun unique_addresses :: "llvm_address list \<Rightarrow> bool" where
+  "unique_addresses (a#as) = (unique_address a as \<and> unique_addresses as)"
+| "unique_addresses [] = True"
+
+fun unique_addresses_rec :: "llvm_identifier list \<Rightarrow> state \<Rightarrow> llvm_address list \<Rightarrow> bool" where
+  "unique_addresses_rec (n#ns) s as = (\<exists>a. register_\<alpha> s (reg n) = Some (addr a) \<and> unique_addresses_rec ns s (a#as))"
+| "unique_addresses_rec []     _ as = unique_addresses as"
+
+fun registers_contain_unique_addresses :: "llvm_identifier list \<Rightarrow> state \<Rightarrow> bool" where
+  "registers_contain_unique_addresses ns s = unique_addresses_rec ns s []"
 
 
 
@@ -148,18 +239,19 @@ method clean_memory = repeat_minus_one thin_tac_mem
 
 method clean_assms = ((elim exE conjE)+)?, (simp only: contract_updates)?; clean_registers?; clean_memory?; (simp only: triv_forall_equality)?
 
+method unfold_shorthands = simp only: registers_contain_unique_addresses.simps unique_addresses.simps unique_addresses_rec.simps unique_address.simps register_contains_value_def register_contains_allocated_address_def register_contains_address_with_value_def HOL.simp_thms(21)
 
 subsection "Subgoal Solving Methods"
 
-method sub_instantiate_register_address = rule asm_rl[of "register_\<alpha> _ _ = Some (addr _)"]; (fastforce | simp); fail
-method sub_memory_allocated = rule asm_rl[of "memory_\<alpha> _ _ \<noteq> None"]; (fastforce | simp); fail
-method sub_register_value = rule asm_rl[of "register_\<alpha> _ _ = Some _"]; (fastforce | simp); fail
-method sub_memory_value = rule asm_rl[of "memory_\<alpha> _ _ = Some (Some _)"]; (fastforce | simp split: if_splits); fail
-method sub_add_poison = (rule asm_rl[of "add_no_poison32 _ _ _"] | rule asm_rl[of "add_no_poison64 _ _ _"]); (fastforce | simp split: if_splits add: word_sless_alt word_sle_eq); fail
-method sub_icmp_same_signs = (rule asm_rl[of "if _ then same_signs32 _ _ else True"] | rule asm_rl[of "if _ then same_signs64 _ _ else True"]); (fastforce | simp split: if_splits add: word_sless_alt word_sle_eq); fail
-method sub_map_of_some = rule asm_rl[of "map_of _ _ = Some _"]; (fastforce | simp); fail
-method sub_distinct_first = rule asm_rl[of "distinct (map fst _)"]; (fastforce | simp); fail
-method sub_some_refl = rule asm_rl[of "Some _ = Some _"]; rule refl; fail
+method sub_instantiate_register_address = rule asm_rl[of "register_\<alpha> _ _ = Some (addr _)"], unfold_shorthands?, (fastforce | simp)?; fail
+method sub_memory_allocated = rule asm_rl[of "memory_\<alpha> _ _ \<noteq> None"], unfold_shorthands?, (fastforce | simp)?; fail
+method sub_register_value = rule asm_rl[of "register_\<alpha> _ _ = Some _"], unfold_shorthands?, (fastforce | simp)?; fail
+method sub_memory_value = rule asm_rl[of "memory_\<alpha> _ _ = Some (Some _)"], unfold_shorthands?, (fastforce | simp split: if_splits)?; fail
+method sub_add_poison = (rule asm_rl[of "add_no_poison32 _ _ _"] | rule asm_rl[of "add_no_poison64 _ _ _"]), unfold_shorthands?, (fastforce | simp split: if_splits add: word_sless_alt word_sle_eq)?; fail
+method sub_icmp_same_signs = (rule asm_rl[of "if _ then same_signs32 _ _ else True"] | rule asm_rl[of "if _ then same_signs64 _ _ else True"]), unfold_shorthands?, (fastforce | simp split: if_splits add: word_sless_alt word_sle_eq)?; fail
+method sub_map_of_some = rule asm_rl[of "map_of _ _ = Some _"], unfold_shorthands?; (fastforce | simp)?; fail
+method sub_distinct_first = rule asm_rl[of "distinct (map fst _)"], unfold_shorthands?; (fastforce | simp)?; fail
+method sub_some_refl = rule asm_rl[of "Some _ = Some _"], unfold_shorthands?; (rule refl)?; fail
 
 method solve_subgoal = sub_instantiate_register_address | sub_memory_allocated | sub_register_value
                      | sub_memory_value | sub_add_poison | sub_icmp_same_signs | sub_map_of_some
@@ -181,7 +273,7 @@ method strat_alloca_dbg = rule asm_rl[of "wp (execute_alloca _ _) _"], strat_ins
 method strat_store_dbg  = rule asm_rl[of "wp (execute_store _ _ _) _"], strat_instr_dbg
 method strat_load_dbg   = rule asm_rl[of "wp (execute_load _ _ _) _"], strat_instr_dbg
 method strat_add_dbg    = rule asm_rl[of "wp (execute_add _ _ _ _ _) _"], strat_instr_dbg
-method strat_icmp_dbg   = rule asm_rl[of "wp (execute_icmp _ _ _ _ _ _) _"], strat_instr_dbg; simp only: compare_values_32.simps compare_values_64.simps
+method strat_icmp_dbg   = rule asm_rl[of "wp (execute_icmp _ _ _ _ _ _) _"], strat_instr_dbg
 
 method unfold_block_instr = rule asm_rl[of "wp (execute_block _ ([], _#_, _) _) _"], rule wp_intro
 method unfold_instr = rule asm_rl[of "wp (execute_instruction _ _) _"], rule wp_intro
@@ -225,19 +317,26 @@ method block_vcg_dbg = block_vcg_step_dbg+
 
 subsection "Multi-Block VCG Methods"
 
-method clean_goal' = (simp (no_asm_simp) split: prod.splits del: register_\<alpha>.simps, intro allI conjI impI)
+method clean_goal' = (simp (no_asm_simp) split: prod.splits del: register_\<alpha>.simps registers_contain_unique_addresses.simps, intro allI conjI impI)
 method clean_goal = (match conclusion in "case _ of (s, r) \<Rightarrow> (case r of return_value _ \<Rightarrow> _ | branch_label _ \<Rightarrow> _)" \<Rightarrow> clean_goal')
 
 method clean_case_prod_goal = simp only: split split: prod.splits; intro allI impI conjI; (simp; fail)?; elim conjE
-
 
 method unfold_execute_blocks_from_until = rule asm_rl[of "hoare _ (execute_blocks_from_until _ _ _) _"], rule hoare_blocks_from_until_intro, sub_map_of_some
 method unfold_verify_blocks_from = rule asm_rl[of "verify_blocks_from _ _ _"], simp
 
 method unfold_verify_function = rule asm_rl[of "verify_function _"], simp del: verify_blocks_from.simps, (intro conjI)?
 
-method vcg_step = elim exE conjE | unfold_verify_function | unfold_verify_blocks_from | unfold_execute_blocks_from_until | clean_goal | block_vcg_step | (force | simp split: if_splits add: word_sless_alt word_sle_eq; fail)
-method vcg_step_dbg = elim exE conjE | unfold_verify_function | unfold_verify_blocks_from | unfold_execute_blocks_from_until | clean_goal | block_vcg_step_dbg | (force | simp split: if_splits add: word_sless_alt word_sle_eq; fail)
+method attempt_endgoal_strat = unfold_shorthands?; (force | simp split: if_splits add: word_sless_alt word_sle_eq)?; fail
+method match_all_but_endgoal = rule asm_rl[of "verify_function _"]
+  | rule asm_rl[of "verify_blocks_from _ _ _"]
+  | rule asm_rl[of "hoare _ _ _"]
+  | rule asm_rl[of "wp _ _"]
+
+method attempt_endgoal = (match_all_but_endgoal | attempt_endgoal_strat); fail
+
+method vcg_step = elim exE conjE | unfold_verify_function | unfold_verify_blocks_from | unfold_execute_blocks_from_until | clean_goal | block_vcg_step | attempt_endgoal
+method vcg_step_dbg = elim exE conjE | unfold_verify_function | unfold_verify_blocks_from | unfold_execute_blocks_from_until | clean_goal | block_vcg_step_dbg | attempt_endgoal
 method vcg = vcg_step+
 method vcg_dbg = vcg_step_dbg+
 
