Semantics.thy
@@ -1,0 +1,198 @@
+theory Semantics
+  imports Structure "HOL-Library.Mapping"
+begin
+
+type_synonym register_state = "(llvm_identifier, llvm_value) mapping"
+
+datatype memory_entry = mem_unset | mem_value llvm_value | mem_freed
+type_synonym mem = "llvm_address \<rightharpoonup> memory_entry"
+
+definition disjoint :: "mem \<Rightarrow> mem \<Rightarrow> bool" where
+  "disjoint h1 h2 \<equiv> dom h1 \<inter> dom h2 = {}"
+
+definition union :: "mem \<Rightarrow> mem \<Rightarrow> mem" ("_ \<union> _" 50) where
+  "(h1 \<union> h2) \<equiv> h1 ++ h2"
+
+definition separating_conjunction :: "(mem \<Rightarrow> bool) \<Rightarrow> (mem \<Rightarrow> bool) \<Rightarrow> (mem \<Rightarrow> bool)" ("_ * _" 50) where
+  "(A * B) h \<equiv> (\<exists>h1 h2. disjoint h1 h2 \<and> h = union h1 h2 \<and> A h1 \<and> B h2)"
+
+definition valid :: "llvm_address \<Rightarrow> mem \<Rightarrow> bool" where
+  "valid l h \<equiv> dom h = {l} \<and> h \<noteq> [l \<mapsto> mem_freed]"
+
+definition contains :: "llvm_address \<Rightarrow> llvm_value \<Rightarrow> (mem \<Rightarrow> bool)" ("_ \<mapsto> _" 50) where
+  "(l \<mapsto> v) h \<equiv> h = [l \<mapsto> mem_value v]"
+
+definition empty :: "mem \<Rightarrow> bool" where
+  "empty h \<equiv> h = Map.empty"
+
+definition prop_empty :: "bool \<Rightarrow> mem \<Rightarrow> bool" where
+  "prop_empty P h \<equiv> empty h \<and> P"
+definition separating_implication :: "(mem \<Rightarrow> bool) \<Rightarrow> (mem \<Rightarrow> bool) \<Rightarrow> (mem \<Rightarrow> bool)" where
+  "separating_implication A B h \<equiv> (\<forall>h'. (disjoint h h' \<and> A h') \<longrightarrow> B (union h h'))"
+
+datatype state = state register_state mem
+
+
+
+definition set_register :: "llvm_identifier \<Rightarrow> llvm_value \<Rightarrow> state \<Rightarrow> state" where
+  "set_register i v s = (case s of state r m \<Rightarrow> state (Mapping.update i v r) m)"
+
+definition get_register :: "llvm_identifier \<Rightarrow> state \<Rightarrow> llvm_value option" where
+  "get_register i s = (case s of state r m \<Rightarrow> Mapping.lookup r i)"
+
+
+
+fun addr_index :: "llvm_address \<Rightarrow> nat" where
+  "addr_index (saddr n) = n"
+| "addr_index (haddr n) = n"
+
+fun is_saddr where
+  "is_saddr (saddr _) = True"
+| "is_saddr _ = False"
+
+fun is_haddr where
+  "is_haddr (haddr _) = True"
+| "is_haddr _ = False"
+
+definition max_address :: "llvm_address set \<Rightarrow> nat" where
+  "max_address d =
+     (if d = {} then 0 else Max (addr_index ` d))"
+
+definition fresh_stack_address :: "mem \<Rightarrow> llvm_address" where
+  "fresh_stack_address h =
+     (let saddrs = {a \<in> dom h. is_saddr a}
+      in saddr (Suc (max_address saddrs)))"
+
+definition fresh_heap_address :: "mem \<Rightarrow> llvm_address" where
+  "fresh_heap_address h =
+     (let haddrs = {a \<in> dom h. is_haddr a}
+      in haddr (Suc (max_address haddrs)))"
+
+
+lemma mem_helper:
+  assumes "finite (dom h)"
+  and "haddr ad = fresh_heap_address h"
+  and "is_haddr x"
+  and "h x = Some y"
+  shows "addr_index x < ad"
+proof (-)
+  have "ad = Suc (if \<forall>x. x \<in> dom h \<longrightarrow> \<not> is_haddr x then 0 else Max (addr_index ` {a \<in> dom h. is_haddr a}))"
+    using assms
+    unfolding fresh_heap_address_def max_address_def
+    by simp
+
+  moreover
+
+  obtain x' where xdef: "haddr x' = x"
+    using assms
+    by (cases x; simp)
+
+  then have "x' \<in> addr_index ` {a \<in> dom h. is_haddr a}"
+    using assms
+    by force
+
+  then have "x' \<le> Max (addr_index ` {a \<in> dom h. is_haddr a})"
+    using assms xdef by simp
+
+  then have "addr_index x \<le> (if \<forall>x. x \<in> dom h \<longrightarrow> \<not> is_haddr x then 0 else Max (addr_index ` {a \<in> dom h. is_haddr a}))"
+    using assms xdef by auto
+
+  ultimately
+
+  show ?thesis by simp
+qed
+
+lemma stack_helper:
+  assumes "finite (dom h)"
+  and "saddr ad = fresh_stack_address h"
+  and "is_saddr x"
+  and "h x = Some y"
+  shows "addr_index x < ad"
+proof (-)
+  have "ad = Suc (if \<forall>x. x \<in> dom h \<longrightarrow> \<not> is_saddr x then 0 else Max (addr_index ` {a \<in> dom h. is_saddr a}))"
+    using assms
+    unfolding fresh_stack_address_def max_address_def
+    by simp
+
+  moreover
+
+  obtain x' where xdef: "saddr x' = x"
+    using assms
+    by (cases x; simp)
+
+  then have "x' \<in> addr_index ` {a \<in> dom h. is_saddr a}"
+    using assms
+    by force
+
+  then have "x' \<le> Max (addr_index ` {a \<in> dom h. is_saddr a})"
+    using assms xdef by simp
+
+  then have "addr_index x \<le> (if \<forall>x. x \<in> dom h \<longrightarrow> \<not> is_saddr x then 0 else Max (addr_index ` {a \<in> dom h. is_saddr a}))"
+    using assms xdef by auto
+
+  ultimately
+
+  show ?thesis by simp
+qed
+
+
+lemma fresh_heap_not_in_dom: "finite (dom h) \<Longrightarrow> fresh_heap_address h \<notin> dom h"
+  using mem_helper unfolding fresh_heap_address_def by force
+
+lemma fresh_stack_not_in_dom: "finite (dom h) \<Longrightarrow> fresh_stack_address h \<notin> dom h"
+  using stack_helper unfolding fresh_stack_address_def by force
+
+
+definition allocate_stack :: "state \<Rightarrow> (state * llvm_address)" where
+  "allocate_stack s \<equiv> (case s of state r m \<Rightarrow> (let a = fresh_stack_address m in (state r (m(a \<mapsto> mem_unset)), a)))"
+
+definition allocate_heap :: "state \<Rightarrow> (state * llvm_address)" where
+  "allocate_heap s \<equiv> (case s of state r m \<Rightarrow> (let a = fresh_heap_address m in (state r (m(a \<mapsto> mem_unset)), a)))"
+
+
+definition "get_memory a s \<equiv> (case s of state r m \<Rightarrow> (case m a of Some (mem_value v) \<Rightarrow> Some v | _ \<Rightarrow> None))"
+
+definition "set_memory a v s \<equiv> (case s of state r m \<Rightarrow> (case m a of None \<Rightarrow> None | Some mem_freed \<Rightarrow> None | _ \<Rightarrow> Some (state r (m(a := Some (mem_value v))))))"
+
+lemma "((a \<mapsto> v) * B) m \<Longrightarrow> get_memory a (state r m) = Some v"
+  unfolding get_memory_def contains_def separating_conjunction_def union_def disjoint_def
+  by (cases "m a"; auto)
+
+lemma "(((a \<mapsto> v) * (b \<mapsto> x)) * (c \<mapsto> y)) m \<Longrightarrow> get_memory a (state r m) = Some v"
+  unfolding get_memory_def contains_def separating_conjunction_def union_def disjoint_def
+  by force
+
+
+lemma "((valid a) * B) m \<Longrightarrow> set_memory a v (state r m) \<noteq> None"
+  unfolding set_memory_def separating_conjunction_def union_def disjoint_def valid_def apply (cases "m a"; auto)
+  subgoal for mv apply (cases mv) apply auto by fastforce
+  done
+
+
+lemma "((valid a) * B) m \<Longrightarrow> set_memory a v (state r m) = Some (state r' m') \<Longrightarrow> r' = r \<and> ((valid a) * B) m' \<and> ((a \<mapsto> v) * B) m'"
+  unfolding set_memory_def contains_def separating_conjunction_def valid_def disjoint_def union_def apply (intro conjI)
+    apply (cases "m a") apply simp apply simp subgoal for mv by (cases mv; simp)
+    apply (cases "m a") apply simp apply simp subgoal for mv apply (cases mv; simp)
+    apply (metis (no_types, lifting) dom_eq_singleton_conv fun_upd_upd insert_disjoint(2) map_add_upd_left map_upd_eqD1
+        memory_entry.distinct(6))
+    by (smt (verit) dom_empty dom_fun_upd fun_upd_None_if_notin_dom fun_upd_upd insert_disjoint(2) map_add_upd
+        map_add_upd_left map_upd_eqD1 memory_entry.distinct(6))
+    apply (cases "m a") apply simp apply simp subgoal for mv apply (cases mv; simp)
+     apply (metis dom_eq_singleton_conv fun_upd_upd insert_disjoint(2) map_add_upd_left)
+    apply auto
+    by (metis domIff dom_eq_singleton_conv fun_upd_upd map_add_upd_left)
+  done
+
+
+
+lemma allocate_heap_sep:
+  assumes "finite (dom h)"
+  assumes "(state r' h', a) = allocate_heap (state r h)"
+  shows "((\<lambda>h1. h1 = h) * (\<lambda>h2. h2 = [a \<mapsto> mem_unset])) h'"
+  unfolding separating_conjunction_def using assms unfolding allocate_stack_def apply auto
+  apply (metis (mono_tags, lifting) Int_insert_right_if0 allocate_heap_def disjoint_def dom_empty dom_fun_upd
+      fresh_heap_not_in_dom inf_bot_right option.distinct(1) snd_conv state.case)
+  by (metis (mono_tags, lifting) allocate_heap_def map_add_empty map_add_upd old.prod.inject state.case state.inject
+      union_def)
+
+end
